case_studies/HamiltonBlum/Blum_Sim1Property.ec
@@ -3,35 +3,24 @@ require import AllCore DBool Bool List Distr Int Aux DJoin.
   
 require import PrArg FSet StdRing StdOrder StdBigop.
 (*---*) import RField RealOrder.
-
+require Djoinmap.
 
 require import Permutation Blum_Basics.
 clone import ZeroKnowledgeTheory as ZKT.
 clone import OneShotSimulator as OSS.
 
+import DJM.
 
-module ZKP(P : HonestProver, V : MaliciousVerifier) = {
-  proc run(Ny : hc_stat, w : hc_wit, b : bool) = {
-    var c,r;
-    c <@ P.commitment(Ny,w);
-    r <@ P.response(b);
-    return (c,r);
-  }
-}.
-
-
-
-module ZKP' = {
+module ZKP = {
   proc run(Ny : hc_stat, w : hc_wit, b : bool) = {
     var c,r,prm,fal,pi_gwco,pi_w;
     prm <$ perm_d K;
     fal <- permute_graph prm Ny;
-    pi_gwco <$ djoinmap Com fal;
+    pi_gwco <@ DJM.main5(fal);
     c <- (unzip1 pi_gwco);
     pi_w <- permute_witness prm w;
     r <- if b then Left (prm, unzip2 pi_gwco) else Right (pi_w, unzip2 (prj_path pi_w pi_gwco));
     return (c, r);
-
   }
 }.
 
@@ -43,9 +32,9 @@ module Sim1(V : RewMaliciousVerifier)  = {
     g <-  p_a;
     bb <$ {0,1};
     if (bb) {
-       r <@ ZKP'.run(p_a, witness, bb);
+       r <@ ZKP.run(p_a, witness, bb);
     }else{
-       r <@ ZKP'.run(compl_graph K, compl_graph_cyc K, bb);
+       r <@ ZKP.run(compl_graph K, compl_graph_cyc K, bb);
     }
     return (bb, r);
   }
@@ -113,13 +102,13 @@ simplify. call V_summitup_ll. call V_challenge_ll. sp.
 conseq (_: true ==> true). progress.  
 call (_:true). sp. 
 seq 1 : (true). rnd. skip. auto. rnd.  skip. smt(@Distr).
-if. call (_:true). wp. simplify. rnd.
+if. call (_:true). wp. simplify. inline*. wp . rnd.
 conseq (_: true ==> true). progress. 
 smt (djoinmap_weight Com_lossless).
  wp.  rnd. skip. smt (perm_d_lossless).
 skip. auto.
 call (_:true).
-wp. simplify. rnd.
+wp. simplify. inline*. wp. rnd.
 conseq (_: true ==> true). progress. 
 smt (djoinmap_weight Com_lossless).
  wp.  rnd. skip. smt (perm_d_lossless).
@@ -140,6 +129,11 @@ end section.
 
 
 section.
+
+op statProb : hc_stat.
+op statWit : hc_wit.
+declare axiom statGood : zk_relation statProb statWit.
+
 declare module V <: RewMaliciousVerifier {-HP, -ZKT.Hyb.Count, -ZKT.Hyb.HybOrcl}.
 declare module D <: ZKDistinguisher {-HP}.
 
@@ -166,8 +160,10 @@ declare axiom rewindable_V_plus :
   islossless V.setState.
 
 
-module Sim1_0(V : RewMaliciousVerifier, D : ZKDistinguisher) = {
-  module ZKP_HP = ZKP(HP,V)
+
+  
+local module Sim1_0(V : RewMaliciousVerifier, D : ZKDistinguisher) = {
+  module ZKP_HP = ZKP
   proc sinit(p_a : hc_stat) : bool * (hc_com * hc_resp) = {
     var  g,bb,r;
     g <- p_a;
@@ -193,22 +189,19 @@ module Sim1_0(V : RewMaliciousVerifier, D : ZKDistinguisher) = {
 
 
 
-module Sim1_1(V : MaliciousVerifier) = {
-  module ZKP_HP = ZKP(HP,V)
+local module Sim1_1(V : MaliciousVerifier) = {
+  module ZKP_HP = ZKP
   proc sinit(p_a : hc_stat, w_a : hc_wit) = {
     var g,bb,r;
     g <- p_a;
-
     bb <$ {0,1};
-
     if (bb) {
        r <@ ZKP_HP.run(p_a, w_a, bb);
     }else{
         r <@ ZKP_HP.run(compl_graph K, w_a, bb);
     }
     return (bb, r);
-  }
- 
+  } 
   proc simulate(pa : hc_stat, wa : hc_wit) : bool * bool  = {
     var b',b,zryb,result, rb;
     (b',zryb) <@ sinit(pa,wa);
@@ -217,8 +210,192 @@ module Sim1_1(V : MaliciousVerifier) = {
     rb <@ D.guess(pa, wa, result);
     return (b = b', rb);
   }
-
 }.
+
+
+
+local module ZKP' = {
+  proc run(Ny : hc_stat, w : hc_wit, b : bool) = {
+    var c,r,prm,fal,pi_w,ko,ok;
+    prm <$ perm_d K;
+    fal <- permute_graph prm Ny;
+    (ok, ko) <@ DJM.main6(fal,prj_path (permute_witness prm w) fal, permute_witness prm w);
+    pi_w <- permute_witness prm w;
+    c <- (unzip1 (rep_path pi_w ok ko));
+    r <- if b then Left (prm, unzip2 (rep_path pi_w ok ko)) else Right (pi_w, unzip2 ko);
+    return (c, r);
+  }
+}.
+
+
+local module Sim1_1'(V : MaliciousVerifier) = {
+  proc sinit(p_a : hc_stat, w_a : hc_wit) = {
+    var g,bb,r;
+    g <- p_a;
+    bb <$ {0,1};
+    if (bb) {
+       r <@ ZKP.run(p_a, w_a, bb);
+    }else{
+        r <@ ZKP'.run(compl_graph K, w_a, bb);
+    }
+    return (bb, r);
+  } 
+  proc simulate(pa : hc_stat, wa : hc_wit) : bool * bool  = {
+    var b',b,zryb,result, rb;
+    (b',zryb) <@ sinit(pa,wa);
+    b <@ V.challenge(pa, zryb.`1);
+    result <@ V.summitup(pa,zryb.`2);
+    rb <@ D.guess(pa, wa, result);
+    return (b = b', rb);
+  }
+}.
+
+
+local module ZKP'' = {
+  proc run(Ny : hc_stat, w : hc_wit, prm: permutation, cs : commitment list)  = {
+    var c,ko,r,pi_w;
+    ko <$ djoinmap Com (nseq K true);
+    pi_w <- permute_witness prm w;
+    c <- (rep_path pi_w cs (unzip1 ko));
+    r <- if false then Left (prm, unzip2 ko) else Right (pi_w, unzip2 ko);
+    return (c, r);
+  }
+}.
+
+
+
+local module ZKP''' = {
+  proc run(Ny : hc_stat, w : hc_wit, prm:permutation, b : bool) = {
+    var c,r,fal,pi_gwco,pi_w;
+    fal <- permute_graph prm Ny;
+    pi_gwco <@ DJM.main5(fal);
+    c <- (unzip1 pi_gwco);
+    pi_w <- permute_witness prm w;
+    r <- if b then Left (prm, unzip2 pi_gwco) else Right (pi_w, unzip2 (prj_path pi_w pi_gwco));
+    return (c, r);
+  }
+}.
+
+
+
+local module BlumUnhider2 : Unhider = {
+  var prm : permutation
+  proc choose() : bool list * bool list = {
+    var fal1,fal2;
+    prm <$ perm_d K;
+    fal1 <- permute_graph prm (compl_graph K);
+    fal2 <- permute_graph prm statProb;
+    return (fal1,fal2);
+  }
+  
+  proc guess(c : commitment list) : bool = {
+    var bb,bb',r,result,dg;
+    bb <$ {0,1};
+    if (bb) {
+       r <@ ZKP'''.run(statProb, statWit, prm,bb);
+    }else{
+        r <@ ZKP''.run(compl_graph K, statWit, prm, c);
+    }    
+    bb' <@ V.challenge(statProb, r.`1);
+    result <@ V.summitup(statProb,r.`2);
+    dg <@ D.guess(statProb, statWit, result);
+    return (bb = bb') /\ dg;
+  }
+}.
+
+
+local module M = {
+  proc main6'(l : bool list, l' : bool list, w : int list) = {
+    var xy;
+    xy <@ DJM.main2(l,l');
+    return  rep_path w xy.`1 xy.`2;
+  }
+}.
+
+local lemma pr1 l l' w a &m : Pr[M.main6'(l,l',w) @ &m : res = a] = mu1 (dapply (fun xx' => rep_path w (fst xx') (snd xx')) ((djoinmap Com l) `*` (djoinmap Com l'))) a.
+progress. byphoare (_: arg = (l,l',w) ==> _). proc.
+inline*.  wp. sp. rnd. skip. progress.
+rewrite dmap1E. simplify.
+have ->: (fun (x : (commitment * opening) list * (commitment * opening) list) => rep_path w{hr} x.`1 x.`2 = a)
+ = (pred1 a \o fun (xx' : (commitment * opening) list * (commitment * opening) list) => rep_path w{hr} xx'.`1 xx'.`2).
+apply fun_ext. move => x. simplify. rewrite /(\o). rewrite /pred1.
+auto. auto. auto. auto.
+qed.
+
+
+local lemma pr2 w l l' a &m : Pr[DJM.main5(rep_path w l' l) @ &m : res = a] = mu1 (djoinmap Com (rep_path w l' l)) a.
+progress. byphoare (_: arg = (rep_path w l' l) ==> _). proc.
+rnd. skip. progress. auto. auto.
+qed.
+
+
+local lemma kikk' w l l' : equiv [DJM.main5 ~ M.main6' : arg{1} = (rep_path w l' l) /\ arg{2} = (l,l',w) ==> res{1} = res{2} ].
+bypr res{1} res{2}. auto.
+progress. rewrite H. rewrite H0.  simplify. rewrite pr1. rewrite pr2. rewrite rep_distr.
+auto.
+qed.
+
+
+local lemma kikk ww l l' : equiv [DJM.main5 ~ DJM.main6 : arg{1} = (rep_path ww l' l) /\ arg{2} = (l,l',ww) ==> res{1} = rep_path ww res.`1{2} res.`2{2} ].
+symmetry.
+transitivity M.main6'
+ (={arg} /\ w{1} = ww ==> rep_path ww res.`1{1} res.`2{1} = res{2})
+ (arg{2} = (rep_path ww l' l) /\ arg{1} = (l,l',ww) ==> ={res}).
+smt().
+smt().
+proc.
+call main12. skip. progress.
+symmetry.
+conseq (kikk' ww l l').
+auto.
+qed.
+
+
+local lemma sim1_1' : equiv [Sim1_1(V).simulate ~ Sim1_1'(V).simulate : ={glob V, arg, glob ZKT.Hyb.Count, glob ZKT.Hyb.HybOrcl} ==> ={res}].
+proc. 
+inline Sim1_1(V).sinit.
+inline Sim1_1'(V).sinit.
+seq 5 5 : (={pa,wa,bb,r,glob V, glob ZKT.Hyb.Count, glob ZKT.Hyb.HybOrcl}).
+seq 4 4 : (={pa,wa,p_a,w_a,bb,glob V, glob ZKT.Hyb.Count, glob ZKT.Hyb.HybOrcl}). 
+rnd. wp. skip. progress.
+if. progress. sim.
+inline Sim1_1(V).ZKP_HP.run.
+inline ZKP'.run. 
+wp. 
+seq 5 5 : (={Ny, w, bb,b0,prm, fal} /\ ={p_a, w_a, pa,wa,b0, glob V, glob Hyb.Count, glob Hyb.HybOrcl} /\ !b0{1} /\ fal{1} = permute_graph prm{1} Ny{1}). wp.  rnd. wp. skip. progress.
+exists* fal{2}. exists* prm{2}. exists* w{2}. elim*. progress.
+call (kikk (permute_witness prm_R w_R) fal_R (prj_path (permute_witness prm_R w_R) fal_R)).
+skip. progress.
+rewrite - prj_rep. auto.
+rewrite  H. simplify. 
+smt(rep_prj).
+call D_guess_prop. 
+call (_:true). call (_:true). wp. skip. progress.
+qed.
+
+
+local lemma sim1'_unhider : equiv [Sim1_1'(V).simulate ~ HidingGame(BlumUnhider2).main : ={glob V,  glob ZKT.Hyb.Count, glob ZKT.Hyb.HybOrcl} /\ arg{1} = (statProb, statWit) /\ arg{2} = true ==> (res.`1{1} /\ res.`2{1}) = res{2}].
+proof. proc.
+inline*. wp. call D_guess_prop. call(_:true). call (_:true). wp. sp. swap {2} 7 -6.
+seq 1 1 : (={glob V, glob Hyb.HybOrcl, glob Hyb.Count,bb} /\ p_a{1} = pa{1} /\ w_a{1} = wa{1} /\ (pa{1},wa{1}) =(statProb,statWit) /\ b{2} = true).    
+rnd. skip. progress.
+case (bb{1} = true).
+rcondt {1} 1. progress. 
+rcondt {2} 7. progress. wp.  rnd. wp. wp. rnd.  skip. progress.  
+sp. wp.  rnd. wp.  rnd{2}. wp. 
+rnd. wp. skip. progress. smt(djoinmap_weight Com_lossless). smt(). 
+rcondf {1} 1. progress. skip. progress. smt().
+rcondf {2} 7. progress. wp.  rnd. wp. wp. rnd.  skip. progress. smt().
+wp.  rnd. wp. rnd. wp. rnd. wp. skip. progress.
+rewrite permute_graph_prop1.
+rewrite lemma9. rewrite /permute_witness. smt (statGood @List). auto.
+have <-: djoinmap Com
+      (prj_path (permute_witness prm0L statWit)
+         (permute_graph prm0L (compl_graph K))) = djoinmap Com (nseq K true).
+rewrite permute_graph_prop1. rewrite lemma9. rewrite /permute_witness. smt (statGood @List). auto. auto.
+smt(rep_map). smt(). smt().
+qed.
+
 
 
 local lemma sim_0_1 (g : hc_stat) (w: hc_wit):  K = size w => zk_relation g w =>
@@ -241,14 +418,14 @@ call (_:true).
 wp. inline*. wp.  call (_:true).
  wp.  rnd.  wp. rnd. wp. skip. progress.
 rewrite H. simplify. auto. 
-seq 1 1 : (={r,bb, glob V,pa,wa, glob ZKT.Hyb.Count, glob ZKT.Hyb.HybOrcl} /\ !bb{1}).
-inline*. 
-seq  13 13 : (
-   !b1{1} /\ b1{1} = b1{2} /\ ={pa,c,wa, HP.pi_w, HP.pi_gwco,bb, glob V, glob ZKT.Hyb.Count, glob ZKT.Hyb.HybOrcl} /\ !bb{1} ).
+seq 1 1 : (={r,bb, glob V,pa,wa, glob ZKT.Hyb.Count, glob ZKT.Hyb.HybOrcl} /\ !bb{1}). 
+inline*.  
+(* seq  13 13 : ( *)
+(*    !b1{1} /\ b1{1} = b1{2} /\ ={pa,c,wa, HP.pi_w, HP.pi_gwco,bb, glob V, glob ZKT.Hyb.Count, glob ZKT.Hyb.HybOrcl} /\ !bb{1} ). *)
 wp.  rnd. wp. 
 rnd  
- (fun (f : permutation) => compose f (inv (mk_perm HP.w{2})))
-  (fun (f : permutation) => compose f (mk_perm HP.w{2})) .
+ (fun (f : permutation) => compose f (inv (mk_perm wa{2})))
+  (fun (f : permutation) => compose f (mk_perm wa{2})) .
 wp. skip. progress.  rewrite /compose.
 simplify. 
 have ->: (prmR \o mk_perm wa{2} \o inv (mk_perm wa{2}))
@@ -276,15 +453,14 @@ rewrite /permute_witness /compose.
 rewrite map_comp.
 rewrite inv_prop3.
 elim ishc. progress. smt(). smt().
-wp. skip. progress. 
-rewrite H.  simplify. auto. 
 call D_guess_prop.
 call (_:true). call (_:true). wp.  skip. progress.
 qed.
 
 
-module Sim1_2(V : MaliciousVerifier) = {
-  module ZKP_HP = ZKP(HP,V)
+
+local module Sim1_2(V : MaliciousVerifier) = {
+  module ZKP_HP = ZKP
   proc sinit(p_a : hc_stat, w_a : hc_wit) = {
     var  g, bb, r;
     g <- p_a;
@@ -309,23 +485,151 @@ module Sim1_2(V : MaliciousVerifier) = {
 }.
 
 
+local module Sim1_2'(V : MaliciousVerifier) = {
+  proc sinit(p_a : hc_stat, w_a : hc_wit) = {
+    var g,bb,r;
+    g <- p_a;
+    bb <$ {0,1};
+    if (bb) {
+       r <@ ZKP.run(p_a, w_a, bb);
+    }else{
+        r <@ ZKP'.run(p_a, w_a, bb);
+    }
+    return (bb, r);
+  } 
+  proc simulate(pa : hc_stat, wa : hc_wit) : bool * bool  = {
+    var b',b,zryb,result, rb;
+    (b',zryb) <@ sinit(pa,wa);
+    b <@ V.challenge(pa, zryb.`1);
+    result <@ V.summitup(pa,zryb.`2);
+    rb <@ D.guess(pa, wa, result);
+    return (b = b', rb);
+  }
+}.
 
-(* ASSUMPTION that commitment scheme is hiding (these could be derived, but would require another round of boiler-plate wrappers).  *)
-op negl, negl2 : real.
-axiom negl_ge0 : 0%r <= negl.
-axiom negl2_ge0 : 0%r <= negl2 < 1%r/4%r.
 
-axiom comm_scheme_hiding1 &m pa wa: 
-   `|Pr[ Sim1_1(V).simulate(pa,wa) @ &m : res.`1 /\ res.`2 ]
-      - Pr[ Sim1_2(V).simulate(pa,wa) @ &m : res.`1 /\ res.`2 ]| 
-   <= negl.
-   
-axiom comm_scheme_hiding2 &m pa :
-  `|Pr[Sim1_0(V,D).simulate(pa) @ &m : res.`1] -  1%r/2%r| <= negl2. 
+local lemma sim12_2' : equiv [Sim1_2(V).simulate ~ Sim1_2'(V).simulate : ={glob V, arg, glob ZKT.Hyb.Count, glob ZKT.Hyb.HybOrcl} ==> ={res}].
+proc. 
+inline Sim1_2(V).sinit.
+inline Sim1_2'(V).sinit.
+seq 5 5 : (={pa,wa,bb,r,glob V, glob ZKT.Hyb.Count, glob ZKT.Hyb.HybOrcl}).
+seq 4 4 : (={pa,wa,p_a,w_a,bb,glob V, glob ZKT.Hyb.Count, glob ZKT.Hyb.HybOrcl}). 
+rnd. wp. skip. progress.
+if. progress. sim.
+inline Sim1_1(V).ZKP_HP.run.
+inline ZKP'.run. 
+wp. 
+seq 5 5 : (={Ny, w, bb,b0,prm, fal} /\ ={p_a, w_a, pa,wa,b0, glob V, glob Hyb.Count, glob Hyb.HybOrcl} /\ !b0{1} /\ fal{1} = permute_graph prm{1} Ny{1}). wp.  rnd. wp. skip. progress.
+exists* fal{2}. exists* prm{2}. exists* w{2}. elim*. progress.
+call (kikk (permute_witness prm_R w_R) fal_R (prj_path (permute_witness prm_R w_R) fal_R)).
+skip. progress.
+smt (prj_rep).
+rewrite  H. simplify. smt (rep_prj).
+call D_guess_prop. 
+call (_:true). call (_:true). wp. skip. progress.
+qed.
+
+
+local lemma sim2'_unhider : equiv [Sim1_2'(V).simulate ~ HidingGame(BlumUnhider2).main : ={glob V,  glob ZKT.Hyb.Count, glob ZKT.Hyb.HybOrcl} /\ arg{1} = (statProb, statWit) /\ arg{2} = false ==> (res.`1{1} /\ res.`2{1}) = res{2}].
+proof. proc.
+inline*. wp. call D_guess_prop. call(_:true). call (_:true). wp. sp. swap {2} 7 -6.
+seq 1 1 : (={glob V, glob Hyb.HybOrcl, glob Hyb.Count,bb} /\ p_a{1} = pa{1} /\ w_a{1} = wa{1} /\ (pa{1},wa{1}) =(statProb,statWit) /\ b{2} = false).
+rnd. skip. progress.
+case (bb{1} = true).
+rcondt {1} 1. progress. 
+rcondt {2} 7. progress. wp.  rnd. wp. wp. rnd.  skip. progress.  
+sp. wp.  rnd. wp.  rnd{2}. wp. 
+rnd.  wp. skip. progress. smt(djoinmap_weight Com_lossless). smt().  
+rcondf {1} 1. progress. skip. progress. smt().
+rcondf {2} 7. progress. wp.  rnd. wp. wp. rnd.  skip. progress.  smt().
+wp.  rnd. wp. rnd. wp. rnd. wp. skip. progress.
+smt(statGood permute_graph_prop3).
+have <-: djoinmap Com
+      (prj_path (permute_witness prm0L statWit)
+         (permute_graph prm0L statProb)) = djoinmap Com (nseq K true).
+smt(statGood permute_graph_prop3).
+smt(rep_map). smt(rep_map). smt(). smt().
+qed.
+
+
+
+local lemma comm_scheme_hiding1 &m: 
+   `|Pr[ Sim1_1(V).simulate(statProb,statWit) @ &m : res.`1 /\ res.`2 ]
+      - Pr[ Sim1_2(V).simulate(statProb,statWit) @ &m : res.`1 /\ res.`2 ]| 
+   <= eps.
+have ->: Pr[Sim1_1(V).simulate(statProb, statWit) @ &m : res.`1 /\ res.`2]
+ = Pr[Sim1_1'(V).simulate(statProb, statWit) @ &m : res.`1 /\ res.`2].
+byequiv(_: ={glob V, arg, glob ZKT.Hyb.Count, glob ZKT.Hyb.HybOrcl} ==> _). conseq sim1_1'.
+auto. auto. auto.
+have ->: Pr[Sim1_1'(V).simulate(statProb, statWit) @ &m : res.`1 /\ res.`2]
+ = Pr[HidingGame(BlumUnhider2).main(true) @ &m : res].
+byequiv(_: ={glob V,  glob ZKT.Hyb.Count, glob ZKT.Hyb.HybOrcl} /\ arg{2} = true /\ arg{1} = (statProb, statWit) ==> _). conseq sim1'_unhider. progress. progress. auto. auto.
+have ->: Pr[Sim1_2(V).simulate(statProb, statWit) @ &m : res.`1 /\ res.`2]
+ = Pr[Sim1_2'(V).simulate(statProb, statWit) @ &m : res.`1 /\ res.`2].
+byequiv(_: ={glob V, arg, glob ZKT.Hyb.Count, glob ZKT.Hyb.HybOrcl} ==> _). conseq sim12_2'.
+auto. auto. auto.
+have ->: Pr[Sim1_2'(V).simulate(statProb, statWit) @ &m : res.`1 /\ res.`2]
+ = Pr[HidingGame(BlumUnhider2).main(false) @ &m : res].
+byequiv(_: ={glob V,  glob ZKT.Hyb.Count, glob ZKT.Hyb.HybOrcl} /\ arg{2} = false /\ arg{1} = (statProb, statWit) ==> _). conseq sim2'_unhider. progress. progress. auto. auto.
+apply (comm_scheme_hiding_eps &m BlumUnhider2).
+qed.
+
+
+local module BlumUnhider : Unhider = {
+ proc choose () : bool list * bool list = {
+    var prm,fal1,fal2;
+    prm <$ perm_d K;
+    fal1 <- permute_graph prm statProb;
+    prm <$ perm_d K;
+    fal2 <- permute_graph prm (compl_graph K);
+    return (fal1,fal2);
+
+ }
+ proc guess(c : commitment list) : bool = {
+   var b : bool;
+   b <@ V.challenge(statProb, c);
+   return b;
+ }
+}.
+
+local lemma zz : equiv [ Sim1_0(V,D).simulate ~ HidingExperiment(BlumUnhider).main : arg{1} = (statProb, statWit) /\ ={glob V} ==> res.`1{1} = res{2} ].
+progress.
+proc. inline*. sp. wp. 
+call {1} (_:true ==> true). apply D_run_ll.
+call {1} (_:true ==> true). apply V_summitup_ll. simplify.
+swap {2} 6 -5.
+call (_:true).  wp.
+seq 1 1 : (bb{1} = b{2} /\   p_a{1} = pa{1} /\
+  g{1} = p_a{1} /\
+  (pa{1} = statProb /\ wa{1} = statWit) /\
+  ={glob V}).
+rnd. skip. progress.
+case (bb{1}). 
+rcondt {1} 1. progress. sp. wp.
+rnd.  wp.  rnd{2}.
+wp. rnd.   wp.  skip. progress. apply perm_d_lossless. 
+rewrite H. simplify. auto.
+rewrite H. simplify. auto.
+smt().
+rcondf {1} 1. progress. sp. wp.
+rnd.  wp.  rnd.
+wp. rnd{2}.   wp.  skip. progress. apply perm_d_lossless.
+rewrite H. simplify. auto. 
+rewrite H. simplify. auto. 
+smt().
+qed.
+
+
+local lemma comm_scheme_hiding2' &m :
+  `|Pr[Sim1_0(V,D).simulate(statProb, statWit) @ &m : res.`1] -  1%r/2%r| <= eps2. 
+have ->: Pr[Sim1_0(V,D).simulate(statProb, statWit) @ &m : res.`1] = Pr[HidingExperiment(BlumUnhider).main() @ &m : res].
+byequiv. conseq zz. progress. smt(). smt(). auto. 
+apply (comm_scheme_hiding_eps2 &m BlumUnhider).
+qed.
 
 
 local module Sim1_3(V : MaliciousVerifier) = {
-  module ZKP_HP = ZKP(HP,V)
+  module ZKP_HP = ZKP
   proc sinit(p_a : hc_stat, w_a : hc_wit) = {
     var  g,bb,r;
     g <- p_a;
@@ -381,7 +685,7 @@ qed.
 
 
 local module Sim1_4(V : MaliciousVerifier) = {
-  module ZKP_HP = ZKP(HP,V)
+  module ZKP_HP = ZKP
   proc simulate(pa : hc_stat, wa : hc_wit) : bool * bool  = {
     var b,result,r,g,bb,rb;
     g <- pa;
@@ -616,47 +920,47 @@ smt (sim_9_pr1 sim_9_pr2).
 qed.
 
 
-local lemma sim1_main &m pa wa:  zk_relation pa wa =>
-   `|Pr[ Sim1_0(V,D).simulate(pa,wa) @ &m : res.`1 /\ res.`2 ]
-      / Pr[ Sim1_0(V,D).simulate(pa,wa) @ &m : res.`1 ]
-         - Pr[ ZKD(HP,V,D).main(pa,wa) @ &m : res ]| 
-  <= 2%r * negl + 20%r * negl2.
+local lemma sim1_main &m:  zk_relation statProb statWit =>
+   `|Pr[ Sim1_0(V,D).simulate(statProb,statWit) @ &m : res.`1 /\ res.`2 ]
+      / Pr[ Sim1_0(V,D).simulate(statProb,statWit) @ &m : res.`1 ]
+         - Pr[ ZKD(HP,V,D).main(statProb,statWit) @ &m : res ]| 
+  <= 2%r * eps + 20%r * eps2.
 proof. move => ishc.
 have ->: 
-  Pr[ ZKD(HP,V,D).main(pa,wa) @ &m : res ]
-  = Pr[ Sim1_9(V).simulate(pa,wa) @ &m : res.`2 ]. 
+  Pr[ ZKD(HP,V,D).main(statProb,statWit) @ &m : res ]
+  = Pr[ Sim1_9(V).simulate(statProb,statWit) @ &m : res.`2 ]. 
  byequiv (_: arg{1} = arg{2} /\ ={glob V, glob HP, glob ZKT.Hyb.Count, glob ZKT.Hyb.HybOrcl}  ==> _). 
  symmetry. conseq sim_9_10. progress;auto. auto. auto. auto.
 have ->: 
-   Pr[Sim1_0(V,D).simulate(pa,wa) @ &m : res.`1 /\ res.`2]
-    = Pr[ Sim1_1(V).simulate(pa,wa) @ &m : res.`1 /\ res.`2 ].
-   byequiv (_: ={glob V, glob ZKT.Hyb.Count, glob ZKT.Hyb.HybOrcl} /\ arg{2} = (pa, wa) /\ arg{1} = (pa, wa) ==> _). 
-conseq (sim_0_1 pa wa _ _ ).   simplify. progress. smt(). auto. auto. auto.
+   Pr[Sim1_0(V,D).simulate(statProb,statWit) @ &m : res.`1 /\ res.`2]
+    = Pr[ Sim1_1(V).simulate(statProb,statWit) @ &m : res.`1 /\ res.`2 ].
+   byequiv (_: ={glob V, glob ZKT.Hyb.Count, glob ZKT.Hyb.HybOrcl} /\ arg{2} = (statProb, statWit) /\ arg{1} = (statProb, statWit) ==> _). 
+conseq (sim_0_1 statProb statWit _ _ ).   simplify. progress. smt(). auto. auto. auto.
 have h: 
-   Pr[Sim1_0(V,D).simulate(pa,wa) @ &m : res.`1]
-    = Pr[ Sim1_1(V).simulate(pa,wa) @ &m : res.`1].
-   byequiv (_: ={glob V, glob ZKT.Hyb.Count, glob ZKT.Hyb.HybOrcl} /\ arg{2} = (pa, wa) /\ arg{1} = (pa, wa) ==> _). conseq (sim_0_1 pa wa _ _). smt(). smt(). auto. auto. auto.
+   Pr[Sim1_0(V,D).simulate(statProb,statWit) @ &m : res.`1]
+    = Pr[ Sim1_1(V).simulate(statProb,statWit) @ &m : res.`1].
+   byequiv (_: ={glob V, glob ZKT.Hyb.Count, glob ZKT.Hyb.HybOrcl} /\ arg{2} = (statProb, statWit) /\ arg{1} = (statProb, statWit) ==> _). conseq (sim_0_1 statProb statWit _ _). smt(). smt(). auto. auto. auto.
 rewrite sim_9_pr3.
 apply (ler_trans (2%r * 
-    `|Pr[Sim1_1(V).simulate(pa,wa) @ &m : res.`1 /\ res.`2] -
-        Pr[Sim1_9(V).simulate(pa,wa) @ &m : res.`2 /\ res.`1]| 
-           + 20%r * negl2)).
+    `|Pr[Sim1_1(V).simulate(statProb,statWit) @ &m : res.`1 /\ res.`2] -
+        Pr[Sim1_9(V).simulate(statProb,statWit) @ &m : res.`2 /\ res.`1]| 
+           + 20%r * eps2)).
 apply main_fin.  split. rewrite Pr[mu_ge0]. auto. rewrite Pr[mu_le1]. auto.
 rewrite Pr[mu_ge0]. auto. rewrite Pr[mu_le1]. auto.
 rewrite Pr[mu_ge0]. auto. rewrite Pr[mu_le1]. auto.
-smt (negl2_ge0). 
+smt (eps2_ge0). 
 rewrite h. rewrite Pr[mu_sub]. auto. auto.
 apply pr_e1. 
 rewrite Pr[mu_ge0]. auto. rewrite Pr[mu_le1]. auto.
-apply comm_scheme_hiding2.
+apply (comm_scheme_hiding2' &m).
 apply pr_e2. 
 rewrite Pr[mu_ge0]. auto. rewrite Pr[mu_le1]. auto.
-apply comm_scheme_hiding2.
-have ->: Pr[Sim1_9(V).simulate(pa, wa) @ &m : res.`2 /\ res.`1] =
- Pr[Sim1_2(V).simulate(pa,wa) @ &m : res.`1 /\ res.`2].
-byequiv (_: (pa,wa) = arg{1} /\ arg{1} = arg{2} 
+apply comm_scheme_hiding2'.
+have ->: Pr[Sim1_9(V).simulate(statProb, statWit) @ &m : res.`2 /\ res.`1] =
+ Pr[Sim1_2(V).simulate(statProb,statWit) @ &m : res.`1 /\ res.`2].
+byequiv (_: (statProb,statWit) = arg{1} /\ arg{1} = arg{2} 
  /\ ={glob V, glob HP, glob ZKT.Hyb.Count, glob ZKT.Hyb.HybOrcl} ==> _). 
-symmetry. conseq (sim_2_9 pa wa ishc). smt(). smt(). auto. auto.
+symmetry. conseq (sim_2_9 statProb statWit ishc). smt(). smt(). auto. auto.
 smt (comm_scheme_hiding1).
 qed.    
 
@@ -693,28 +997,28 @@ qed.
 
 
 (* conditional indistinguishability  *)
-lemma sim1_error &m (p : hc_stat) (ww : hc_wit) :
+lemma sim1_error &m :
    islossless D.guess =>
    islossless V.summitup =>
-   zk_relation p ww =>  
-    `|Pr[RD(Sim1(V), D).run(p, ww) @ &m : fst res.`2 /\ res.`1] /
-         Pr[Sim1(V).run(p) @ &m : fst res] 
-              - Pr[ ZKD(HP,V,D).main(p,ww) @ &m : res ]| <= 2%r * negl + 20%r * negl2.
+   zk_relation statProb statWit =>  
+    `|Pr[RD(Sim1(V), D).run(statProb, statWit) @ &m : fst res.`2 /\ res.`1] /
+         Pr[Sim1(V).run(statProb) @ &m : fst res] 
+              - Pr[ ZKD(HP,V,D).main(statProb,statWit) @ &m : res ]| <= 2%r * eps + 20%r * eps2.
 progress.
-have ->: Pr[RD(Sim1(V), D).run(p, ww) @ &m : fst res.`2 /\ res.`1]
- = Pr[ Sim1_0(V,D).simulate(p,ww) @ &m : res.`1 /\ res.`2 ].
-progress. byequiv (_: (p,ww) = arg{1} /\ arg{1} = arg{2}
+have ->: Pr[RD(Sim1(V), D).run(statProb, statWit) @ &m : fst res.`2 /\ res.`1]
+ = Pr[ Sim1_0(V,D).simulate(statProb,statWit) @ &m : res.`1 /\ res.`2 ].
+progress. byequiv (_: (statProb,statWit) = arg{1} /\ arg{1} = arg{2}
  /\ ={glob V,  glob ZKT.Hyb.Count, glob ZKT.Hyb.HybOrcl} ==> _).  proc. simplify.
-seq 1 3 : (={glob ZKT.Hyb.Count, glob ZKT.Hyb.HybOrcl} /\ (p = a{1} ) /\
+seq 1 3 : (={glob ZKT.Hyb.Count, glob ZKT.Hyb.HybOrcl} /\ (statProb = a{1} ) /\
   (a{1} = pa{2} /\ w{1} = wa{2}) /\ r.`2{1} = result{2} /\ (r{1}.`1  <=> b{2} = b'{2}) /\ (b{2} = b'{2} => ={glob V})  ).
 inline Sim1(V).run. wp. sp. simplify.
 seq 4 3 :   (={Hyb.Count.c, Hyb.HybOrcl.l, Hyb.HybOrcl.l0} /\
-  p = a{1} /\
+  statProb = a{1} /\
   (a{1} = pa{2} /\ w{1} = wa{2}) /\
   ={result} /\
   (b0{1} = b'{1} <=> b{2} = b'{2}) /\ (b{2} = b'{2} => ={glob V})).  call (_:true). call (_:true).
 seq 1 0 : (  pa{1} = a{1} /\
-  (p = a{1} /\ ww = w{1}) /\
+  (statProb = a{1} /\ statWit = w{1}) /\
   (a{1} = pa{2} /\ w{1} = wa{2}) /\
   ={glob V, Hyb.Count.c, Hyb.HybOrcl.l, Hyb.HybOrcl.l0}). 
 elim rewindable_V_plus.
@@ -727,7 +1031,7 @@ seq 1 1 :     (p_a{2} = pa{2} /\
   p_a{1} = pa{1} /\
   g{1} = p_a{1} /\
   pa{1} = a{1} /\
-  (p = a{1} /\ ww = w{1}) /\
+  (statProb = a{1} /\ statWit = w{1}) /\
   (a{1} = pa{2} /\ w{1} = wa{2}) /\
   ={glob V, Hyb.Count.c, Hyb.HybOrcl.l, Hyb.HybOrcl.l0,bb}). rnd.  skip. progress.
 if. progress. wp.  rnd.  wp. rnd. wp. skip. progress.
@@ -741,21 +1045,21 @@ apply s7. skip. smt().
 case (b{2} = b'{2}). 
 call D_guess_prop. skip.  progress. 
 call {1} H. call {2} H. skip. smt(). auto. auto.
-rewrite (sim110 p ww &m H).
-apply (sim1_main  &m  p ww). assumption.
+rewrite (sim110 statProb statWit &m H).
+apply (sim1_main  &m). assumption.
 qed.
 
 (* probability of a "success"-event  *)
-lemma sim1_succ &m stat : 
- 1%r/2%r - negl2 <= Pr[Sim1(V).run(stat) @ &m : res.`1].
+lemma sim1_succ &m  : 
+ 1%r/2%r - eps2 <= Pr[Sim1(V).run(statProb) @ &m : res.`1].
 progress.
-have ->: Pr[Sim1(V).run(stat) @ &m : res.`1] = 
- Pr[Sim1_0(V,D).simulate(stat, witness) @ &m : res.`1] .
-rewrite (sim110 stat  witness &m).
+have ->: Pr[Sim1(V).run(statProb) @ &m : res.`1] = 
+ Pr[Sim1_0(V,D).simulate(statProb, statWit) @ &m : res.`1] .
+rewrite (sim110 statProb statWit &m).
 apply D_run_ll. auto.
-have f : `|Pr[Sim1_0(V, D).simulate(stat,  witness) @ &m : res.`1] - 1%r / 2%r|
- <= negl2. 
-apply comm_scheme_hiding2. smt().
+have f : `|Pr[Sim1_0(V, D).simulate(statProb,  statWit) @ &m : res.`1] - 1%r / 2%r|
+ <= eps2. 
+apply comm_scheme_hiding2'. smt().
 qed.
 
 end section.
