case_studies/HamiltonBlum/Blum_ZeroKnowledge.ec
@@ -1,24 +1,30 @@
 pragma Goals:printall.
 require import AllCore DBool Bool List Distr Int Aux DJoin.
-require import Permutation Blum_Basics Blum_Sim1Property.
-
-import OSS.
-clone import ZKT.SequentialComposition.
-clone import Statistical with op epsilon <- 2%r * negl + 20%r * negl2,
-                              op sigma <- (1%r/2%r - negl2).
-
+require import Permutation Blum_Basics.
+require Blum_Sim1Property.
 
 
 require RewBasics.
 clone import RewBasics as Rew with type sbits <- sbits.
 
+op stat : hc_stat.
+op wit : hc_wit.
+
+clone import Blum_Sim1Property as BSP with op statProb <- stat,
+                                     op statWit <- wit.
+
+import OSS.
+clone import ZKT.SequentialComposition.
+clone import Statistical with op epsilon <- 2%r * eps + 20%r * eps2,
+                              op sigma <- (1%r/2%r - eps2).
+
 
 section.
 
+
+declare axiom stat_wit : zk_relation stat wit.
 declare module V <: RewMaliciousVerifier{-HP, -ZKT.Hyb.HybOrcl,-ZKT.Hyb.Count}.
 declare module D <: ZKDistinguisher{-HP,-ZKT.Hyb.HybOrcl,-ZKT.Hyb.Count}.
-
-
 
 declare axiom Sim1_run_ll : forall (V0 <: RewMaliciousVerifier), islossless V0.challenge => islossless V0.summitup => islossless Sim1(V0).run.
 declare axiom V_summitup_ll : islossless V.summitup. 
@@ -39,53 +45,49 @@ declare axiom rewindable_V_plus :
            Pr[V.setState(b) @ &m : glob V = x] = 1%r) /\
          islossless V.setState).
 
+                                     
 
-      
-lemma hc_statistical_zk stat wit  &m:
+lemma hc_statistical_zk   &m:
         zk_relation stat wit => 
         let real_prob = Pr[ZKReal(HP, V, D).run(stat, wit) @ &m : res] in
         let ideal_prob = Pr[ZKIdeal(SimN(Sim1), V, D).run(stat, wit) @ &m : res] in
-          `|ideal_prob - real_prob| <= (2%r * negl + 20%r * negl2) + 2%r * (1%r- (1%r/2%r - negl2)) ^ OSS.N.
+          `|ideal_prob - real_prob| <= (2%r * eps + 20%r * eps2) + 2%r * (1%r- (1%r/2%r - eps2)) ^ OSS.N.
 proof.
 progress.
-apply (statistical_zk HP Sim1  V D _ _ _ _ _ _ _ _ _ _  stat wit &m _). apply Sim1_run_ll. apply V_summitup_ll. apply V_challenge_ll. apply P_response_ll. apply P_commitment_ll.
+apply (statistical_zk HP Sim1 V D _ _ _ _ _ _ _ stat wit &m). apply Sim1_run_ll. apply V_summitup_ll. apply V_challenge_ll. apply P_response_ll. apply P_commitment_ll.
 apply D_guess_ll. 
 proc*. call D_guess_prop. skip.  auto.
 move => x.
 conseq (sim1_rew_ph V _ _ _ _ _  x.`1).  auto. auto.
 apply V_summitup_ll. apply V_challenge_ll. apply P_response_ll. apply P_commitment_ll.
 apply (rewindable_A_plus V). apply rewindable_V_plus.
-progress.
-apply (sim1_error V D  _ _  _ _ _  _ &m0 p w  _ );auto.  apply V_summitup_ll. 
+apply (sim1_error stat_wit V D  _ _  _ _ _  _ &m   _ );auto.   apply V_summitup_ll. 
 apply D_guess_ll. apply V_summitup_ll. apply V_challenge_ll. 
 conseq D_guess_prop. auto. apply (rewindable_A_plus V). apply rewindable_V_plus.  apply D_guess_ll. apply V_summitup_ll.
-progress.
-apply (sim1_succ V D _ _ _ _ _ _ &m0 stat0 ).  apply V_summitup_ll. apply D_guess_ll. apply V_summitup_ll.
-apply V_challenge_ll. 
- progress. 
+progress. 
+apply (sim1_succ stat_wit V D _ _ _ _ _ _ &m  ).  apply V_summitup_ll. apply D_guess_ll. apply V_summitup_ll.
+apply V_challenge_ll.
+ progress.
 conseq D_guess_prop. auto.
-apply (rewindable_A_plus V). apply rewindable_V_plus. 
+apply (rewindable_A_plus V). apply rewindable_V_plus.
 auto.
 qed.
 
-
-
-
-lemma hc_statistical_zk_iter stat wit &m:
+lemma hc_statistical_zk_iter &m:
         zk_relation stat wit =>
         let real_prob = Pr[ZKRealAmp(HP, V, D).run(stat, wit) @ &m : res] in
         let ideal_prob = Pr[ZKIdeal(SimAmp(SimN(Sim1)), V, D).run(stat, wit) @ &m : res] in
-          `|ideal_prob - real_prob| <= ZKT.n%r * ((2%r * negl + 20%r * negl2) + 2%r * (1%r- (1%r/2%r - negl2)) ^ OSS.N).
+          `|ideal_prob - real_prob| <= ZKT.n%r * ((2%r * eps + 20%r * eps2) + 2%r * (1%r- (1%r/2%r - eps2)) ^ OSS.N).
 progress.
-apply (zk_seq HP (SimN(Sim1)) V D _ _ _ _ _ _ _ &m  ((2%r * negl + 20%r * negl2) + 2%r * (1%r- (1%r/2%r - negl2)) ^ OSS.N) stat wit). 
+apply (zk_seq HP (SimN(Sim1)) V D _ _ _ _ _ _ _ &m  ((2%r * eps + 20%r * eps2) + 2%r * (1%r- (1%r/2%r - eps2)) ^ OSS.N) stat wit). 
 progress.  
 apply (simn_simulate_ll V0). auto. auto.
 apply V_summitup_ll. apply V_challenge_ll. apply P_response_ll.
 apply P_commitment_ll. apply D_guess_ll.
 apply D_guess_prop.
-smt(negl2_ge0 negl_ge0 N_pos @RealExp).
+smt(eps2_ge0 eps_ge0 N_pos @RealExp).
 progress.
-apply (statistical_zk HP Sim1  V (Di(D, SimN(Sim1), V)) _ _ _ _ _ _ _ _ _ _  stat wit &n _).
+apply (statistical_zk HP Sim1  V (Di(D, SimN(Sim1), V))  _ _ _ _ _ _ _ stat wit &n ).
 apply Sim1_run_ll.
 apply V_summitup_ll. apply V_challenge_ll. apply P_response_ll.
 apply P_commitment_ll. 
@@ -102,7 +104,7 @@ call (sim1_rew_ph V _ _ _ _ _ x.`1).  apply V_summitup_ll.
 apply V_challenge_ll. apply P_response_ll.
 apply P_commitment_ll. 
 apply (rewindable_A_plus V). apply rewindable_V_plus.  skip. auto. progress.
-rewrite (sim1_error V (Di(D, SimN(Sim1), V))).
+rewrite (sim1_error stat_wit V (Di(D, SimN(Sim1), V))).
 apply V_summitup_ll.  
 proc. 
 call D_guess_ll. sp.
@@ -117,7 +119,7 @@ while (true) (ZKT.n - ZKT.Hyb.HybOrcl.l). progress. wp.
 call (simn_simulate_ll V).  apply V_challenge_ll. apply V_summitup_ll.  skip. smt().
 skip. smt(). apply V_summitup_ll. auto.
 progress.
-rewrite (sim1_succ V D _ _ _ _  _  _ &m0 stat0). 
+rewrite (sim1_succ stat_wit V D _ _ _ _  _  _ &n ). 
 apply V_summitup_ll.
 apply D_guess_ll. 
 apply V_summitup_ll.
